module Experimental.DependentTypes.DeepEmbedding.Alternative3 where

open import Data.Nat renaming (_≟_ to _≟nat_)
open import Data.Product
open import Data.Unit hiding (_≟_)
open import Function using (_∘_)
open import Relation.Nullary
open import Relation.Binary.PropositionalEquality

open import Model.BaseCategory as M
open import Model.CwF-Structure as M hiding (_,,_)
open import Model.Type.Constant as M
open import Model.Type.Function as M hiding (_⇛_)
open import Model.Type.Product as M hiding (_⊠_)

import Experimental.DependentTypes.Model.IdentityType.AlternativeTerm as M

open import Experimental.DependentTypes.DeepEmbedding.Syntax.AnnotatedIdentity
open import MSTT.TCMonad


-- TODO: Use of de Bruijn indices is incorrect, e.g. shift needed when extending context.

is-yes : ∀ {ℓ} {A : Set ℓ} → Dec A → TCM ⊤
is-yes (yes _) = return tt
is-yes (no _)  = type-error ""

_≟tm_ : TmExpr → TmExpr → TCM ⊤
_≟ty_ : TyExpr → TyExpr → TCM ⊤

(ann t ∈ T) ≟tm (ann s ∈ S) = (t ≟tm s) >> (T ≟ty S)
var x ≟tm var y = is-yes (x ≟nat y)
lam T b ≟tm lam S c = (T ≟ty S) >> (b ≟tm c)
(t1 ∙ s1) ≟tm (t2 ∙ s2) = (t1 ≟tm t2) >> (s1 ≟tm s2)
lit n ≟tm lit m = is-yes (n ≟nat m)
suc ≟tm suc = return tt
plus ≟tm plus = return tt
true ≟tm true = return tt
false ≟tm false = return tt
if c t f ≟tm if c' t' f' = (c ≟tm c') >> (t ≟tm t') >> (f ≟tm f')
pair t1 s1 ≟tm pair t2 s2 = (t1 ≟tm t2) >> (s1 ≟tm s2)
fst p1 ≟tm fst p2 = p1 ≟tm p2
snd p1 ≟tm snd p2 = p1 ≟tm p2
refl t ≟tm refl s = t ≟tm s
t ≟tm s = type-error ""

Nat ≟ty Nat = return tt
Bool ≟ty Bool = return tt
(T1 ⇛ S1) ≟ty (T2 ⇛ S2) = (T1 ≟ty T2) >> (S1 ≟ty S2)
(T1 ⊠ S1) ≟ty (T2 ⊠ S2) = (T1 ≟ty T2) >> (S1 ≟ty S2)
Id T1 t1 s1 ≟ty Id T2 t2 s2 = (T1 ≟ty T2) >> (t1 ≟tm t2) >> (s1 ≟tm s2)
T ≟ty S = type-error ""

lookup-var : ℕ → CtxExpr → TCM TyExpr
lookup-var x ◇ = type-error ""
lookup-var zero    (Γ ,, T) = return T
lookup-var (suc x) (Γ ,, T) = lookup-var x Γ

infer-tm : TmExpr → CtxExpr → TCM TyExpr
infer-tm (ann t ∈ S) Γ = do
  T ← infer-tm t Γ
  T ≟ty S
  return S
infer-tm (var x) Γ = lookup-var x Γ
infer-tm (lam T b) Γ = do
  S ← infer-tm b (Γ ,, T)
  return (T ⇛ S)
infer-tm (t1 ∙ t2) Γ = do
  T1 ← infer-tm t1 Γ
  fun-ty T S ← is-fun-ty T1
  T2 ← infer-tm t2 Γ
  T2 ≟ty T
  return S
infer-tm (lit n) Γ = return Nat
infer-tm suc Γ = return (Nat ⇛ Nat)
infer-tm plus Γ = return (Nat ⇛ Nat ⇛ Nat)
infer-tm true Γ = return Bool
infer-tm false Γ = return Bool
infer-tm (if c t f) Γ = do
  C ← infer-tm c Γ
  C ≟ty Bool
  T ← infer-tm t Γ
  F ← infer-tm f Γ
  T ≟ty F
  return T
infer-tm (pair t1 t2) Γ = do
  T1 ← infer-tm t1 Γ
  T2 ← infer-tm t2 Γ
  return (T1 ⊠ T2)
infer-tm (fst p) Γ = do
  P ← infer-tm p Γ
  prod-ty T S ← is-prod-ty P
  return T
infer-tm (snd p) Γ = do
  P ← infer-tm p Γ
  prod-ty T S ← is-prod-ty P
  return S
infer-tm (refl t) Γ = do
  T ← infer-tm t Γ
  return (Id T t t)

check-ty : TyExpr → CtxExpr → TCM ⊤
check-ty Nat Γ = return tt
check-ty Bool Γ = return tt
check-ty (T ⇛ S) Γ = check-ty T Γ >> check-ty S Γ
check-ty (T ⊠ S) Γ = check-ty T Γ >> check-ty S Γ
check-ty (Id R t s) Γ = do
  T ← infer-tm t Γ
  T ≟ty R
  S ← infer-tm s Γ
  S ≟ty R


HasType : TmExpr → TyExpr → CtxExpr → Set
HasType t T Γ = infer-tm t Γ ≡ ok T

IsValidTy : TyExpr → CtxExpr → Set
IsValidTy T Γ = check-ty T Γ ≡ ok tt

IsValidCtx : CtxExpr → Set
IsValidCtx ◇ = ⊤
IsValidCtx (Γ ,, T) = IsValidCtx Γ × IsValidTy T Γ

conversion : {t : TmExpr} {T S : TyExpr} {Γ : CtxExpr}→
             HasType t T Γ → .(T ≟ty S ≡ ok tt) → HasType t S Γ
conversion = {!!}

tm-has-valid-ty : {t : TmExpr} {T : TyExpr} {Γ : CtxExpr} →
                  HasType t T Γ → IsValidTy T Γ
tm-has-valid-ty = {!!}

valid-ty-has-valid-ctx : {T : TyExpr} {Γ : CtxExpr} →
                         IsValidTy T Γ → IsValidCtx Γ
valid-ty-has-valid-ctx = {!!}

tm-has-valid-ctx : {t : TmExpr} {T : TyExpr} {Γ : CtxExpr} →
                   HasType t T Γ → IsValidCtx Γ
tm-has-valid-ctx {t} {T} = valid-ty-has-valid-ctx {T} ∘ tm-has-valid-ty {t}


interpret-ctx : (Γ : CtxExpr) → IsValidCtx Γ → Ctx ★
interpret-ty : (T : TyExpr) {Γ : CtxExpr} → .(IsValidTy T Γ) → {vΓ : IsValidCtx Γ} → Ty (interpret-ctx Γ vΓ)
interpret-tm : (t : TmExpr) (T : TyExpr) (Γ : CtxExpr) →
               HasType t T Γ →
               (vT : IsValidTy T Γ) (vΓ : IsValidCtx Γ) →
               Tm (interpret-ctx Γ vΓ) (interpret-ty T vT)
≟ty-sound : (T S : TyExpr) → (T ≟ty S ≡ ok tt) →
            {Γ : CtxExpr} {vΓ : IsValidCtx Γ} {vT : IsValidTy T Γ} {vS : IsValidTy S Γ} →
            interpret-ty T vT {vΓ} ≅ᵗʸ interpret-ty S vS
≟tm-sound : (t s : TmExpr) → (t ≟tm s ≡ ok tt) →
            {Γ : CtxExpr} {vΓ : IsValidCtx Γ} {T : TyExpr} {vT : IsValidTy T Γ} →
            (vt : HasType t T Γ) (vs : HasType s T Γ) →
            interpret-tm t T Γ vt vT vΓ ≅ᵗᵐ interpret-tm s T Γ vs vT vΓ


interpret-ctx ◇ vΓ = M.◇
interpret-ctx (Γ ,, T) (vΓ , vT) = interpret-ctx Γ vΓ M.,, interpret-ty T vT

interpret-ty Nat _ = M.Nat'
interpret-ty Bool _ = M.Bool'
interpret-ty (T ⇛ S) {Γ} vT with check-ty T Γ in vT
interpret-ty (T ⇛ S) {Γ} vS | ok tt = interpret-ty T vT M.⇛ interpret-ty S vS
interpret-ty (T ⊠ S) {Γ} vT with check-ty T Γ in vT
interpret-ty (T ⊠ S) {Γ} vS | ok tt = interpret-ty T vT M.⊠ interpret-ty S vS
interpret-ty (Id R t s) {Γ} vT with infer-tm t Γ in vt
interpret-ty (Id R t s) {Γ} vR  | ok T with T ≟ty R in T=R | infer-tm s Γ in vs
interpret-ty (Id R t s) {Γ} S=R | ok T | ok tt | ok S =
  M.Id (interpret-tm t R Γ t∈R (tm-has-valid-ty {t} t∈R) _)
       (interpret-tm s R Γ s∈R (tm-has-valid-ty {s} s∈R) _)
  where
    t∈R : HasType t R Γ
    t∈R = conversion {t} vt T=R

    s∈R : HasType s R Γ
    s∈R = conversion {s} vs S=R

interpret-tm (ann t ∈ S) T Γ vt vT vΓ with infer-tm t Γ in vt'
interpret-tm (ann t ∈ S) T Γ vt vT vΓ | ok R with R ≟ty S in R=S
interpret-tm (ann t ∈ S) .S Γ refl vS vΓ | ok R | ok tt = interpret-tm t S Γ (conversion {t} vt' R=S) vS vΓ
interpret-tm (var zero) T (Γ ,, .T) refl vT (vΓ , vS) = ι[ {!!} ] ξ
interpret-tm (var (suc x)) T (Γ ,, S) vt vT (vΓ , vS) = ι[ {!!} ] (interpret-tm (var x) T Γ vt {!!} vΓ [ π ]')
interpret-tm (lam x t) T Γ vt vT vΓ = {!!}
interpret-tm (f ∙ t) T Γ vt vT vΓ = {!!}
interpret-tm (lit n) .Nat Γ refl vT vΓ = const n
interpret-tm suc .(Nat ⇛ Nat) Γ refl vT vΓ = suc'
interpret-tm plus .(Nat ⇛ Nat ⇛ Nat) Γ refl vT vΓ = nat-sum
interpret-tm true .Bool Γ refl vT vΓ = true'
interpret-tm false .Bool Γ refl vT vΓ = false'
interpret-tm (if c t f) T Γ vt vT vΓ = {!!}
interpret-tm (pair t s) T Γ vt vT vΓ = {!!}
interpret-tm (fst p) T Γ vt vT vΓ = {!!}
interpret-tm (snd p) T Γ vt vT vΓ = {!!}
interpret-tm (refl t) S Γ vt vS vΓ with infer-tm t Γ
interpret-tm (refl t) .(Id T t t) Γ refl vS vΓ | ok T = {!!}

≟ty-sound = {!!}

≟tm-sound = {!!}
