module Experimental.LogicalFramework.Instances.Trivial where

open import Data.Empty
open import Data.Maybe
open import Data.Unit
open import Relation.Binary.PropositionalEquality

import Model.BaseCategory as M
import Model.Modality as M

open import Experimental.LogicalFramework.MSTT.Parameter.ModeTheory
open import Experimental.LogicalFramework.MSTT.Parameter.TypeExtension
open import Experimental.LogicalFramework.MSTT.Parameter


record TrivMode : Set where
  constructor â˜…

triv-mt : ModeTheory
MTBasis.Mode (ModeTheory.mtb triv-mt) = TrivMode
MTBasis.NonTrivModality (ModeTheory.mtb triv-mt) _ _ = âŠ¥
MTBasis.mode-eq? (ModeTheory.mtb triv-mt) _ _ = just refl
MTBasis.non-triv-mod-eq? (ModeTheory.mtb triv-mt) () ()
MTBasis.âŸ¦_âŸ§mode (ModeTheory.mtb triv-mt) â˜… = M.â˜…
MTBasis.âŸ¦_âŸ§non-triv-mod (ModeTheory.mtb triv-mt) ()
MTComposition._â“œnon-triv_ (ModeTheory.mtc triv-mt) () ()
MTComposition.âŸ¦â“œâŸ§-non-triv-sound (ModeTheory.mtc triv-mt) () ()
MTCompositionLaws.mod-non-triv-assoc (ModeTheory.mtc-laws triv-mt) () () ()
MTTwoCell.TwoCell (ModeTheory.mt2 triv-mt) MTBasis.ğŸ™ MTBasis.ğŸ™ = âŠ¤
MTTwoCell.id-cell (ModeTheory.mt2 triv-mt) {Î¼ = MTBasis.ğŸ™} = tt
MTTwoCell._â“£-vert_ (ModeTheory.mt2 triv-mt) {Î¼ = MTBasis.ğŸ™} {Ï = MTBasis.ğŸ™} {Îº = MTBasis.ğŸ™} _ _ = tt
MTTwoCell._â“£-hor_ (ModeTheory.mt2 triv-mt) {Î¼1 = MTBasis.ğŸ™} {MTBasis.ğŸ™} {MTBasis.ğŸ™} {MTBasis.ğŸ™} _ _ = tt
MTTwoCell.two-cell-eq? (ModeTheory.mt2 triv-mt) {Î¼ = MTBasis.ğŸ™} {MTBasis.ğŸ™} tt tt = just refl
MTTwoCell.âŸ¦_âŸ§two-cell (ModeTheory.mt2 triv-mt) {Î¼ = MTBasis.ğŸ™} {MTBasis.ğŸ™} tt = M.id-cell

open ModeTheory triv-mt public hiding (id-cell)

-- The following type of id-cell works better with Agda's type inference
id-cell : TwoCell ğŸ™ ğŸ™
id-cell = ModeTheory.id-cell triv-mt {Î¼ = ğŸ™}


triv-ty-ext : TyExt triv-mt
TyExt.TyExtCode triv-ty-ext _ _ = âŠ¥
TyExt._â‰Ÿty-code_ triv-ty-ext () ()
TyExt.show-ty-code triv-ty-ext ()
TyExt.âŸ¦ triv-ty-ext âŸ§ty-code ()
TyExt.sem-ty-code-natural triv-ty-ext ()
TyExt.sem-ty-code-cong triv-ty-ext ()


triv-mstt : MSTT-Parameter
MSTT-Parameter.â„³ triv-mstt = triv-mt
MSTT-Parameter.ğ’¯ triv-mstt = triv-ty-ext
