open import Model.BaseCategory

module Experimental.DependentTypes.Model.SigmaType {C : BaseCategory} where

open import Data.Product using (Σ; Σ-syntax; proj₁; proj₂; _×_) renaming (_,_ to [_,_])
open import Function using (id)
open import Relation.Binary.PropositionalEquality hiding ([_]; naturality)

open import Model.CwF-Structure.Context
open import Model.CwF-Structure.Type
open import Model.CwF-Structure.Term
open import Model.CwF-Structure.ContextExtension

open BaseCategory C

private
  variable
    Γ Δ : Ctx C
    T T' S S' : Ty Γ


Sigma : (T : Ty Γ) → Ty (Γ ,, T) → Ty Γ
Sigma T S ⟨ x , γ ⟩ = Σ[ t ∈ T ⟨ x , γ ⟩ ] S ⟨ x , [ γ , t ] ⟩
Sigma T S ⟪ f , e ⟫ [ t , s ] = [ T ⟪ f , e ⟫ t , S ⟪ f , to-Σ-ty-eq T e (ty-cong-2-1 T hom-idʳ) ⟫ s ]
ty-cong (Sigma T S) e = to-Σ-ty-eq S (ty-cong T e) (ty-cong-2-1 S (trans hom-idʳ e))
ty-id (Sigma T S) = to-Σ-ty-eq S (ty-id T) (trans (ty-cong-2-1 S hom-idˡ) (ty-id S))
ty-comp (Sigma T S) = to-Σ-ty-eq S (ty-comp T) (ty-cong-2-2 S hom-idʳ)

{-
sigma-cong : {T T' : Ty Γ} {S : Ty (Γ ,, T)} {S' : Ty (Γ ,, T')}
             (e : T ≅ᵗʸ T') → ιc⁻¹[ ,,-cong e ] S ≅ᵗʸ S' → Sigma T S ≅ᵗʸ Sigma T' S'
func (from (sigma-cong {S = S} T=T' S=S')) [ t , s ] = [ func (from T=T') t , func (from S=S') (ty-ctx-subst S ((cong [ _ ,_]) (sym (eq (isoˡ T=T') t))) s) ]
naturality (from (sigma-cong {T' = T'} {S = S} {S' = S'} T=T' S=S')) {f = f} {eγ = eγ} {t = [ t , s ]} = to-Σ-ty-eq S' (naturality (from T=T')) (
  begin
    S' ⟪ hom-id , _ ⟫ S' ⟪ f , _ ⟫ func (from S=S') (S ⟪ hom-id , _ ⟫ s)
  ≡⟨ ty-cong-2-1 S' hom-idʳ ⟩
    S' ⟪ f , to-Σ-ty-eq T' eγ (trans (ty-cong-2-1 T' hom-idʳ) (naturality (from T=T'))) ⟫ func (from S=S') (S ⟪ hom-id , _ ⟫ s)
  ≡⟨ naturality (from S=S') ⟩
    func (from S=S') (S ⟪ f , _ ⟫ S ⟪ hom-id , _ ⟫ s)
  ≡⟨ cong (func (from S=S')) (ty-cong-2-2 S (trans hom-idˡ (sym hom-idʳ))) ⟩
    func (from S=S') (S ⟪ hom-id , _ ⟫ S ⟪ f , _ ⟫ s) ∎)
  where open ≡-Reasoning
func (to (sigma-cong T=T' S=S')) [ t' , s' ] = [ func (to T=T') t' , func (to S=S') s' ]
naturality (to (sigma-cong {S = S} T=T' S=S')) = to-Σ-ty-eq S (naturality (to T=T')) (trans (ty-cong-2-1 S hom-idʳ) (naturality (to S=S')))
eq (isoˡ (sigma-cong {S = S} T=T' S=S')) [ t , s ] = to-Σ-ty-eq S (eq (isoˡ T=T') t) (
  begin
    S ⟪ hom-id , _ ⟫ func (to S=S') (func (from S=S') (S ⟪ hom-id , _ ⟫ s))
  ≡⟨ cong (S ⟪ hom-id , _ ⟫_) (eq (isoˡ S=S') _) ⟩
    S ⟪ hom-id , _ ⟫ S ⟪ hom-id , _ ⟫ s
  ≡⟨ ty-cong-2-1 S hom-idʳ ⟩
    S ⟪ hom-id , _ ⟫ s
  ≡⟨ ty-id S ⟩
    s ∎)
  where open ≡-Reasoning
eq (isoʳ (sigma-cong {Γ = Γ} {T' = T'} {S = S} {S' = S'} T=T' S=S')) [ t' , s' ] = to-Σ-ty-eq S' (eq (isoʳ T=T') t') (
  begin
    S' ⟪ hom-id , _ ⟫ func (from S=S') (S ⟪ hom-id , _ ⟫ func (to S=S') s')
  ≡⟨ cong (λ x → S' ⟪ hom-id , _ ⟫ func (from S=S') x) (ty-cong S refl) ⟩
    S' ⟪ hom-id , _ ⟫ func (from S=S') (S ⟪ hom-id , _ ⟫ func (to S=S') s')
  ≡˘⟨ cong (S' ⟪ hom-id , _ ⟫_) (naturality (from S=S')) ⟩
    S' ⟪ hom-id , _ ⟫ S' ⟪ hom-id , to-Σ-ty-eq T' (ctx-id Γ) (trans (ty-cong-2-1 T' hom-idʳ) (trans (strong-ty-id T') (sym (eq (isoʳ T=T') t')))) ⟫ func (from S=S') (func (to S=S') s')
  ≡⟨ ty-cong-2-1 S' hom-idʳ ⟩
    S' ⟪ hom-id , _ ⟫ func (from S=S') (func (to S=S') s')
  ≡⟨ ty-id S' ⟩
    func (from S=S') (func (to S=S') s')
  ≡⟨ eq (isoʳ S=S') s' ⟩
    s' ∎)
  where open ≡-Reasoning
-}

sigma-natural : (σ : Δ ⇒ Γ) {T : Ty Γ} {S : Ty (Γ ,, T)} → Sigma T S [ σ ] ≅ᵗʸ Sigma (T [ σ ]) (S [ σ ⊹ ])
func (from (sigma-natural σ)) p = p
naturality (from (sigma-natural σ {S = S})) = (cong [ _ ,_]) (ty-cong S refl)
func (to (sigma-natural σ)) p = p
naturality (to (sigma-natural σ {S = S})) = (cong [ _ ,_]) (ty-cong S refl)
eq (isoˡ (sigma-natural σ)) _ = refl
eq (isoʳ (sigma-natural σ)) _ = refl

tm-subst : Tm Γ T → (Γ ⇒ Γ ,, T)
tm-subst {Γ = Γ} {T = T} t = ⟨ id-subst Γ , t [ id-subst Γ ]' ∈ T ⟩

pair : (t : Tm Γ T) → Tm Γ (S [ tm-subst t ]) → Tm Γ (Sigma T S)
pair t s ⟨ x , γ ⟩' = [ t ⟨ x , γ ⟩' , s ⟨ x , γ ⟩' ]
naturality (pair {S = S} t s) f eγ = to-Σ-ty-eq S (naturality t f eγ)
                                                  (trans (ty-cong-2-1 S hom-idʳ) (naturality s f eγ))

fst : Tm Γ (Sigma T S) → Tm Γ T
fst p ⟨ x , γ ⟩' = proj₁ (p ⟨ x , γ ⟩')
naturality (fst p) f eγ = cong proj₁ (naturality p f eγ)

snd : (p : Tm Γ (Sigma T S)) → Tm Γ (S [ tm-subst (fst p) ])
snd p ⟨ x , γ ⟩' = proj₂ (p ⟨ x , γ ⟩')
naturality (snd {S = S} p) f eγ = trans (sym (ty-cong-2-1 S hom-idʳ))
                                        (proj₂ (from-Σ-ty-eq S (naturality p f eγ)))

{-
⊠-bimap : (T ↣ T') → (S ↣ S') → (T ⊠ S ↣ T' ⊠ S')
func (⊠-bimap η φ) [ t , s ] = [ func η t , func φ s ]
naturality (⊠-bimap η φ) = cong₂ [_,_] (naturality η) (naturality φ)

⊠-cong : T ≅ᵗʸ T' → S ≅ᵗʸ S' → T ⊠ S ≅ᵗʸ T' ⊠ S'
from (⊠-cong T=T' S=S') = ⊠-bimap (from T=T') (from S=S')
to (⊠-cong T=T' S=S') = ⊠-bimap (to T=T') (to S=S')
eq (isoˡ (⊠-cong T=T' S=S')) [ t , s ] = cong₂ [_,_] (eq (isoˡ T=T') t) (eq (isoˡ S=S') s)
eq (isoʳ (⊠-cong T=T' S=S')) [ t , s ] = cong₂ [_,_] (eq (isoʳ T=T') t) (eq (isoʳ S=S') s)

pair : Tm Γ T → Tm Γ S → Tm Γ (T ⊠ S)
pair t s ⟨ x , γ ⟩' = [ t ⟨ x , γ ⟩' , s ⟨ x , γ ⟩' ]
naturality (pair t s) f eγ = cong₂ [_,_] (naturality t f eγ) (naturality s f eγ)

fst : Tm Γ (T ⊠ S) → Tm Γ T
fst p ⟨ x , γ ⟩' = proj₁ (p ⟨ x , γ ⟩')
naturality (fst p) f eγ = cong proj₁ (naturality p f eγ)

snd : Tm Γ (T ⊠ S) → Tm Γ S
snd p ⟨ x , γ ⟩' = proj₂ (p ⟨ x , γ ⟩')
naturality (snd p) f eγ = cong proj₂ (naturality p f eγ)

pair-cong : {t t' : Tm Γ T} {s s' : Tm Γ S} → t ≅ᵗᵐ t' → s ≅ᵗᵐ s' → pair t s ≅ᵗᵐ pair t' s'
eq (pair-cong t=t' s=s') γ = cong₂ [_,_] (eq t=t' γ) (eq s=s' γ)

fst-cong : {p p' : Tm Γ (T ⊠ S)} → p ≅ᵗᵐ p' → fst p ≅ᵗᵐ fst p'
eq (fst-cong p=p') γ = cong proj₁ (eq p=p' γ)

snd-cong : {p p' : Tm Γ (T ⊠ S)} → p ≅ᵗᵐ p' → snd p ≅ᵗᵐ snd p'
eq (snd-cong p=p') γ = cong proj₂ (eq p=p' γ)

module _
  {T : Ty Γ} {T' : Ty Γ} {S : Ty Γ} {S' : Ty Γ}
  (T=T' : T ≅ᵗʸ T') (S=S' : S ≅ᵗʸ S')
  where
  pair-ι : (t : Tm Γ T') (s : Tm Γ S') → ι[ ⊠-cong T=T' S=S' ] pair t s ≅ᵗᵐ pair (ι[ T=T' ] t) (ι[ S=S' ] s)
  eq (pair-ι t s) _ = refl

  fst-ι : (p : Tm Γ (T' ⊠ S')) → ι[ T=T' ] fst p ≅ᵗᵐ fst (ι[ ⊠-cong T=T' S=S' ] p)
  eq (fst-ι p) _ = refl

  snd-ι : (p : Tm Γ (T' ⊠ S')) → ι[ S=S' ] snd p ≅ᵗᵐ snd (ι[ ⊠-cong T=T' S=S' ] p)
  eq (snd-ι p) _ = refl

module _ {T : Ty Γ} {S : Ty Γ} (σ : Δ ⇒ Γ) where
  ⊠-natural : (T ⊠ S) [ σ ] ≅ᵗʸ (T [ σ ]) ⊠ (S [ σ ])
  func (from ⊠-natural) = id
  naturality (from ⊠-natural) = refl
  func (to ⊠-natural) = id
  naturality (to ⊠-natural) = refl
  eq (isoˡ ⊠-natural) _ = refl
  eq (isoʳ ⊠-natural) _ = refl

  pair-natural : (t : Tm Γ T) (s : Tm Γ S) → (pair t s) [ σ ]' ≅ᵗᵐ ι[ ⊠-natural ] (pair (t [ σ ]') (s [ σ ]'))
  eq (pair-natural t s) _ = refl

  fst-natural : (p : Tm Γ (T ⊠ S)) → (fst p) [ σ ]' ≅ᵗᵐ fst (ι⁻¹[ ⊠-natural ] (p [ σ ]'))
  eq (fst-natural p) _ = refl

  snd-natural : (p : Tm Γ (T ⊠ S)) → (snd p) [ σ ]' ≅ᵗᵐ snd (ι⁻¹[ ⊠-natural ] (p [ σ ]'))
  eq (snd-natural p) _ = refl

module _ (t : Tm Γ T) (s : Tm Γ S) where
  β-⊠-fst : fst (pair t s) ≅ᵗᵐ t
  eq β-⊠-fst _ = refl

  β-⊠-snd : snd (pair t s) ≅ᵗᵐ s
  eq β-⊠-snd _ = refl

η-⊠ : (p : Tm Γ (T ⊠ S)) →
      p ≅ᵗᵐ pair (fst p) (snd p)
eq (η-⊠ p) _ = refl
-}
