{-# OPTIONS --without-K #-}

--------------------------------------------------
-- The yoneda embedding and yoneda lemma
--------------------------------------------------

open import Categories

module CwF-Structure.Yoneda {C : Category} where

open import Function using (_âˆ˜_)
open import Level renaming (zero to lzero; suc to lsuc)
import Relation.Binary.Reasoning.Setoid as SetoidReasoning
open import Relation.Binary.PropositionalEquality
  hiding ([_]; naturality) renaming (refl to â‰¡-refl; sym to â‰¡-sym; trans to â‰¡-trans; setoid to â‰¡-setoid)

open import Helpers
open import CwF-Structure.Contexts

open Category C

private
  variable
    x y : Ob
    r : Level
    Î“ : Ctx C â„“ r


-- Yoneda embedding
ğ•ª : Ob â†’ Ctx C 0â„“ 0â„“
setoid (ğ•ª x) y = â‰¡-setoid (Hom y x)
rel (ğ•ª x) f g = g âˆ™ f
rel-cong (ğ•ª x) f = cong (_âˆ™ f)
rel-id (ğ•ª x) _ = hom-idÊ³
rel-comp (ğ•ª x) _ _ _ = â‰¡-sym âˆ™assoc

-- The Yoneda lemma
to-ğ•ªâ‡’* : Î“ âŸ¨ x âŸ© â†’ ğ•ª x â‡’ Î“
func (to-ğ•ªâ‡’* {Î“ = Î“} Î³) f = Î“ âŸª f âŸ« Î³
func-cong (to-ğ•ªâ‡’* {Î“ = Î“} Î³) â‰¡-refl = ctxâ‰ˆ-refl Î“
naturality (to-ğ•ªâ‡’* {Î“ = Î“} Î³) f = ctxâ‰ˆ-sym Î“ (rel-comp Î“ _ f Î³)

from-ğ•ªâ‡’* : ğ•ª x â‡’ Î“ â†’ Î“ âŸ¨ x âŸ©
from-ğ•ªâ‡’* Ïƒ = func Ïƒ hom-id

ğ•ª-to-âˆ˜-from : (Ïƒ : ğ•ª x â‡’ Î“) â†’ to-ğ•ªâ‡’* (from-ğ•ªâ‡’* Ïƒ) â‰…Ë¢ Ïƒ
eq (ğ•ª-to-âˆ˜-from {Î“ = Î“} Ïƒ) f =
  begin
    Î“ âŸª f âŸ« func Ïƒ hom-id
  â‰ˆâŸ¨ naturality Ïƒ hom-id âŸ©
    func Ïƒ (hom-id âˆ™ f)
  â‰ˆâŸ¨ func-cong Ïƒ hom-idË¡ âŸ©
    func Ïƒ f âˆ
  where open SetoidReasoning (setoid Î“ _)

ğ•ª-from-âˆ˜-to : (Î³ : Î“ âŸ¨ x âŸ©) â†’ from-ğ•ªâ‡’* {Î“ = Î“} (to-ğ•ªâ‡’* Î³) â‰ˆ[ Î“ ]â‰ˆ Î³
ğ•ª-from-âˆ˜-to {Î“ = Î“} Î³ = rel-id Î“ Î³

-- Proving that the Yoneda embedding is fully faithful
to-ğ•ªâ‡’ğ•ª : Hom x y â†’ ğ•ª x â‡’ ğ•ª y
to-ğ•ªâ‡’ğ•ª = to-ğ•ªâ‡’*

from-ğ•ªâ‡’ğ•ª : ğ•ª x â‡’ ğ•ª y â†’ Hom x y
from-ğ•ªâ‡’ğ•ª = from-ğ•ªâ‡’*

ğ•ª-from-âˆ˜-to' : (f : Hom x y) â†’ from-ğ•ªâ‡’ğ•ª (to-ğ•ªâ‡’ğ•ª f) â‰¡ f
ğ•ª-from-âˆ˜-to' f = hom-idÊ³

ğ•ª-to-âˆ˜-from' : (Ïƒ : ğ•ª x â‡’ ğ•ª y) â†’ to-ğ•ªâ‡’ğ•ª (from-ğ•ªâ‡’ğ•ª Ïƒ) â‰…Ë¢ Ïƒ
ğ•ª-to-âˆ˜-from' Ïƒ = ğ•ª-to-âˆ˜-from Ïƒ

-- Functoriality of the Yoneda embedding
ğ•ª-refl : to-ğ•ªâ‡’ğ•ª hom-id â‰…Ë¢ id-subst (ğ•ª x)
eq ğ•ª-refl _ = hom-idË¡

ğ•ª-comp : (f : Hom x y) (Î³ : Î“ âŸ¨ y âŸ©) â†’ to-ğ•ªâ‡’* {Î“ = Î“} Î³ âŠš to-ğ•ªâ‡’ğ•ª f â‰…Ë¢ to-ğ•ªâ‡’* (Î“ âŸª f âŸ« Î³)
eq (ğ•ª-comp {Î“ = Î“} f Î³) g = rel-comp Î“ g f Î³
